Prelude/NativeLib.bpl
@@ -14,18 +14,7 @@ function getTarsBySrcs(Seq ref): ref;
 function getTarsBySrcs_inverse(ref): Seq ref;
 axiom (forall i: Seq ref :: { getTarsBySrcs(i) } getTarsBySrcs_inverse(getTarsBySrcs(i)) == i);
 
-function surj_tar_model($s: HeapType, $t: HeapType): bool
-{
-(
-forall $o: ref :: $o!=null && read($t, $o, alloc) && dtype($o) == REL$RELSchema ==>
-	(exists $i: ref :: dtype($i) == ER$ERSchema && $i != null && read($s, $i, alloc) && getTarsBySrcs(Seq#Singleton($i))==$o)
-)
-&&
-(
-forall $o: ref :: $o!=null && read($t, $o, alloc) && dtype($o) == REL$Relation ==>
-	(exists $i: ref :: (dtype($i) == ER$Entity || dtype($i)==ER$Relship) && $i != null && read($s, $i, alloc) && getTarsBySrcs(Seq#Singleton($i))==$o)
-)
-}
+
 
 
 procedure NTransientLink#setRule
